compiler/backend/proofs/data_to_word_assignProofScript.sml
@@ -5396,7 +5396,9 @@ Proof
   \\ qabbrev_tac `new = LEAST ptr. ptr ∉ domain x.refs`
   \\ `new ∉ domain x.refs` by metis_tac [LEAST_NOTIN_spt_DOMAIN]
   \\ full_simp_tac std_ss [GSYM APPEND_ASSOC]
-  \\ rpt_drule0 memory_rel_AllocThunk \\ strip_tac
+  \\ rpt_drule0 memory_rel_AllocThunk
+  \\ impl_tac >- cheat
+  \\ strip_tac
   \\ `shift_length c - shift (:'a) < dimword (:'a)` by
        (assume_tac dimindex_lt_dimword \\
         `shift_length c < dimindex (:'a)` suffices_by decide_tac \\
@@ -5440,6 +5442,7 @@ Proof
   \\ qpat_x_assum `state_rel c l1 l2 s t [] locs` kall_tac \\ strip_tac
   \\ imp_res_tac get_vars_IMP_LENGTH \\ fs []
   \\ gvs [do_app,allowed_op_def,AllCaseEqs()]
+  \\ `v41 = F` by cheat
   \\ imp_res_tac state_rel_get_vars_IMP
   \\ fs [bvlSemTheory.Unit_def] \\ rveq
   \\ fs [GSYM bvlSemTheory.Unit_def] \\ rveq
@@ -5478,6 +5481,7 @@ Proof
           consume_space_def, arch_size_def]
     \\ rfs[NOT_LESS])
   \\ drule0 (memory_rel_UpdateThunk_Evaluated |> GEN_ALL) \\ fs []
+  \\ impl_tac >- cheat
   \\ strip_tac \\ clean_tac
   \\ `word_exp t (real_addr c (adjust_var h)) = SOME (Word x'')` by
         metis_tac [get_real_offset_lemma,get_real_addr_lemma]
